cp

pulse/ulib/experimental/Steel.Semantics.Hoare.fst
@@ -15,6 +15,9 @@
 *)
 module Steel.Semantics.Hoare
 
+open FStar.Tactics
+
+
 (*
  * This module provides a semantic model for a combined effect of
  * divergence, state, and parallel composition of atomic actions.
@@ -35,7 +38,8 @@ module Steel.Semantics.Hoare
 
 /// Disabling projectors because we don't use them and they increase the typechecking time
 
-#push-options "--fuel  0 --ifuel 2 --z3rlimit 20 --print_implicits --print_universes" //--__temp_no_proj Steel.Semantics.Hoare"
+#push-options "--fuel  0 --ifuel 2 --z3rlimit 20 --print_implicits --print_universes \
+  --using_facts_from 'Prims FStar.Pervasives Steel.Semantics.Hoare'"
 
 
 (**** Begin state defn ****)
@@ -55,7 +59,7 @@ let transitive #a (equals:a -> a -> prop) =
   forall x y z. x `equals` y /\ y `equals` z ==> x `equals` z
 
 let associative #a (equals: a -> a -> prop) (f: a -> a -> a)=
-  forall x y z.{:pattern f x (f y z) \/ f (f x y) z}
+  forall x y z. //{:pattern f x (f y z) \/ f (f x y) z}
     f x (f y z) `equals` f (f x y) z
 
 let commutative #a (equals: a -> a -> prop) (f: a -> a -> a) =
@@ -286,12 +290,14 @@ let l_post (#st:st) (#a:Type) (pre:st.hprop) (post:post st a) = fp_prop2 pre pos
 
 (**** Begin interface of actions ****)
 
+/// Actions are essentially state transformers that preserve frames
+
 let preserves_frame (#st:st) (pre post:st.hprop) (m0 m1:st.mem) =
   forall (frame:st.hprop).
     st.interp (st.locks_invariant m0 `st.star` (pre `st.star` frame)) (st.heap_of_mem m0) ==>
     (st.interp (st.locks_invariant m1 `st.star` (post `st.star` frame)) (st.heap_of_mem m1) /\
      (forall (f_frame:fp_prop frame). f_frame (st.heap_of_mem m0) <==> f_frame (st.heap_of_mem m1)))
-  
+
 let preserves_frame_trans (#st:st)
   (hp1 hp2 hp3:st.hprop) (m1 m2 m3:st.mem)
 : Lemma
@@ -311,13 +317,6 @@ let action_t (#st:st) (#a:Type) (pre:st.hprop) (post:post st a) (lpre:l_pre pre)
     st.interp (st.locks_invariant m1 `st.star` (post x)) (st.heap_of_mem m1) /\
     lpost (st.heap_of_mem m0) x (st.heap_of_mem m1) /\
     preserves_frame pre (post x) m0 m1)
-
-
-// /// Actions preserve frames AND all fp_props of frames
-
-
-// let action_t (#st:st) (fp:st.hprop) (a:Type) (fp':a -> st.hprop) =
-//   f:action0 fp a fp'{is_frame_preserving f}
 
 
 (**** End interface of actions ****)
@@ -376,6 +375,9 @@ let par_lpost (#st:st) (#aL:Type) (#preL:st.hprop) (#postL:post st aL)
 = fun h0 (xL, xR) h1 -> lpreL h0 /\ lpreR h0 /\ lpostL h0 xL h1 /\ lpostR h0 xR h1
 
 
+/// We never use projectors from m, so don't bother generating, typechecking, and verifying them
+
+#push-options "--__temp_no_proj Steel.Semantics.Hoare"
 noeq
 type m (st:st) : a:Type u#a -> pre:st.hprop -> post:post st a -> l_pre pre -> l_post pre post -> Type =
   | Ret:
@@ -386,12 +388,12 @@ type m (st:st) : a:Type u#a -> pre:st.hprop -> post:post st a -> l_pre pre -> l_
     m st a (post x) post (return_lpre #_ #_ #post x lpost) lpost
 
   | Bind:
-    #a:Type ->
+    #a:Type u#a ->
     #pre:st.hprop ->
     #post_a:post st a ->
     #lpre_a:l_pre pre ->
     #lpost_a:l_post pre post_a ->
-    #b:Type ->
+    #b:Type u#a ->
     #post_b:post st b ->
     #lpre_b:(x:a -> l_pre (post_a x)) ->
     #lpost_b:(x:a -> l_post (post_a x) post_b) ->
@@ -402,7 +404,7 @@ type m (st:st) : a:Type u#a -> pre:st.hprop -> post:post st a -> l_pre pre -> l_
       (bind_lpost lpre_a lpost_a lpost_b)
 
   | Act:
-    #a:Type ->
+    #a:Type u#a ->
     #pre:st.hprop ->
     #post:post st a ->
     #lpre:l_pre pre ->
@@ -424,13 +426,13 @@ type m (st:st) : a:Type u#a -> pre:st.hprop -> post:post st a -> l_pre pre -> l_
       (frame_lpost lpre lpost f_frame)
 
   | Par:
-    #aL:Type ->
+    #aL:Type u#a ->
     #preL:st.hprop ->
     #postL:post st aL ->
     #lpreL:l_pre preL ->
     #lpostL:l_post preL postL ->
     mL:m st aL preL postL lpreL lpostL ->
-    #aR:Type ->
+    #aR:Type u#a ->
     #preR:st.hprop ->
     #postR:post st aR ->
     #lpreR:l_pre preR ->
@@ -441,7 +443,7 @@ type m (st:st) : a:Type u#a -> pre:st.hprop -> post:post st a -> l_pre pre -> l_
       (par_lpost lpreL lpostL lpreR lpostR)
 
   | Weaken:
-    #a:Type ->
+    #a:Type u#a ->
     #pre:st.hprop ->
     #post:post st a ->
     #lpre:l_pre pre ->
@@ -453,7 +455,7 @@ type m (st:st) : a:Type u#a -> pre:st.hprop -> post:post st a -> l_pre pre -> l_
        (forall h0 x h1. lpost h0 x h1 ==> wlpost h0 x h1)) ->
     m st a pre post lpre lpost ->
     m st a pre post wlpre wlpost
-
+#pop-options
 
 (**** End definition of the computation AST ****)
 
@@ -461,20 +463,20 @@ type m (st:st) : a:Type u#a -> pre:st.hprop -> post:post st a -> l_pre pre -> l_
 (**** Stepping relation ****)
 
 
-/// All steps preserve frames and their fp props
+/// All steps preserve frames
 
 noeq
 type step_result (#st:st) (a:Type u#a) (q:post st a) =
   | Step:
-    old_state:st.mem ->
-    step_pre:st.hprop ->
-    fpost:st.hprop ->
-    new_state:st.mem{
-      st.interp (st.locks_invariant new_state `st.star` fpost) (st.heap_of_mem new_state) /\
-      preserves_frame step_pre fpost old_state new_state} ->
-    lpre:l_pre fpost{lpre (st.heap_of_mem new_state)} ->
-    lpost:l_post fpost q ->
-    m st a fpost q lpre lpost ->
+    prev_pre:st.hprop ->
+    prev_state:st.mem ->
+    next_pre:st.hprop ->
+    next_state:st.mem{
+      st.interp (st.locks_invariant next_state `st.star` next_pre) (st.heap_of_mem next_state) /\
+      preserves_frame prev_pre next_pre prev_state next_state} ->
+    lpre:l_pre next_pre{lpre (st.heap_of_mem next_state)} ->
+    lpost:l_post next_pre q ->
+    m st a next_pre q lpre lpost ->
     nat ->
     step_result a q
 
@@ -527,9 +529,9 @@ let step_ens (#st:st)
   (state:st.mem)
 : step_result a post -> Type0
 = fun r ->
-  let Step state1 pre1 next_pre next_state next_lpre next_lpost _ _ = r in
-  state1 == state /\
+  let Step pre1 state1 next_pre next_state next_lpre next_lpost _ _ = r in
   pre1 == pre /\
+  state1 == state /\
   weaker_pre lpre next_lpre state next_state /\
   stronger_post lpost next_lpost state next_state
 
@@ -543,8 +545,8 @@ type step_t =
   f:m st a pre post lpre lpost ->
   state:st.mem ->
   Div (step_result a post)
-      (step_req f state)
-      (step_ens f state)
+  (step_req f state)
+  (step_ens f state)
 
 
 (**** Auxiliary lemmas ****)
@@ -564,53 +566,16 @@ let equals_ext_right (#st:st) (p q r:st.hprop)
     p `st.star` r;
   }
 
-let ac_reasoning_for_frame (#st:st) (p q r s:st.hprop)
-: Lemma
-  (((p `st.star` (q `st.star` r)) `st.star` s) `st.equals`
-   ((p `st.star` q) `st.star` (r `st.star` s)))
-= calc (st.equals) {
-    (p `st.star` (q `st.star` r)) `st.star` s;
-       (st.equals) { }
-    ((p `st.star` q) `st.star` r) `st.star` s;
-       (st.equals) { }
-    (p `st.star` q) `st.star` (r `st.star` s);
-   }
-
-let frame_fp_props_for_frame (#st:st) (frame frame':st.hprop) (f_frame':fp_prop frame')
-  (state next_state:st.mem)
-: Lemma
-  (requires
-    f_frame' (st.heap_of_mem state) /\
-    (forall (hp:fp_prop (frame' `st.star` frame)).
-       hp (st.heap_of_mem state) <==> hp (st.heap_of_mem next_state)))
-  (ensures
-    f_frame' (st.heap_of_mem next_state) /\
-    (forall (hp:fp_prop frame).
-       hp (st.heap_of_mem state) <==> hp (st.heap_of_mem next_state)))
-= ()
-
-let ac_reasoning_for_par_right (#st:st) (p q r s:st.hprop)
-: Lemma
-  (((p `st.star` (q `st.star` r)) `st.star` s) `st.equals`
-   ((p `st.star` r) `st.star` (q `st.star` s)))
-= calc (st.equals) {
-    (p `st.star` (q `st.star` r)) `st.star` s;
-       (st.equals) { equals_ext_right p (q `st.star` r) (r `st.star` q) }
-    (p `st.star` (r `st.star` q)) `st.star` s;
-       (st.equals) { }
-    ((p `st.star` r) `st.star` q) `st.star` s;
-       (st.equals) { }
-    (p `st.star` r) `st.star` (q `st.star` s);
-  }
-
 /// Lemma frame_post_for_par is used in the par proof
 ///
 /// E.g. in the par rule, when L takes a step, we can frame the requires of R
-///   by adding it to the frame used in the stepping relation
+///   by using the preserves_frame property of the stepping relation
 ///
-/// However we also need to frame the ensures of R, basically, we need:
+/// However we also need to frame the ensures of R, for establishing stronger_post
 ///
-/// forall x h_final. postR old_state x h_final <==> postR next_state x h_final
+/// Basically, we need:
+///
+/// forall x h_final. postR prev_state x h_final <==> postR next_state x h_final
 ///
 /// (the proof only requires the reverse implication, but we can prove iff)
 ///
@@ -627,42 +592,42 @@ let inst_heap_prop_for_par (#st:st) (#a:Type) (#pre:st.hprop) (#post:post st a)
                    lpost (st.heap_of_mem state) x final_state
 
 let frame_post_for_par_tautology (#st:st)
-  (#a:Type) (#preF:st.hprop) (#postF:post st a) (lpostF:l_post preF postF)
+  (#a:Type) (#pre_f:st.hprop) (#post_f:post st a) (lpost_f:l_post pre_f post_f)
   (m0:st.mem)
-: Lemma (inst_heap_prop_for_par lpostF m0 (st.heap_of_mem m0))
+: Lemma (inst_heap_prop_for_par lpost_f m0 (st.heap_of_mem m0))
 = ()
 
 let frame_post_for_par_aux (#st:st)
-  (preS:st.hprop) (postS:st.hprop) (m0 m1:st.mem)
-  (#a:Type) (#preF:st.hprop) (#postF:post st a) (lpostF:l_post preF postF)
+  (pre_s post_s:st.hprop) (m0 m1:st.mem)
+  (#a:Type) (#pre_f:st.hprop) (#post_f:post st a) (lpost_f:l_post pre_f post_f)
 : Lemma
   (requires
-    preserves_frame preS postS m0 m1 /\
-    st.interp (st.locks_invariant m0 `st.star` preS `st.star` preF) (st.heap_of_mem m0))
+    preserves_frame pre_s post_s m0 m1 /\
+    st.interp (st.locks_invariant m0 `st.star` (pre_s `st.star` pre_f)) (st.heap_of_mem m0))
   (ensures
-    inst_heap_prop_for_par lpostF m0 (st.heap_of_mem m0) <==> inst_heap_prop_for_par lpostF m0 (st.heap_of_mem m1))
+    inst_heap_prop_for_par lpost_f m0 (st.heap_of_mem m0) <==>
+    inst_heap_prop_for_par lpost_f m0 (st.heap_of_mem m1))
 = ()
 
 let frame_post_for_par (#st:st)
-  (preS:st.hprop) (postS:st.hprop) (m0 m1:st.mem)
-  (#a:Type) (#preF:st.hprop) (#postF:post st a) (lpreF:l_pre preF) (lpostF:l_post preF postF)
+  (pre_s post_s:st.hprop) (m0 m1:st.mem)
+  (#a:Type) (#pre_f:st.hprop) (#post_f:post st a) (lpre_f:l_pre pre_f) (lpost_f:l_post pre_f post_f)
 : Lemma
   (requires
-    preserves_frame preS postS m0 m1 /\
-    st.interp (st.locks_invariant m0 `st.star` preS `st.star` preF) (st.heap_of_mem m0))
+    preserves_frame pre_s post_s m0 m1 /\
+    st.interp (st.locks_invariant m0 `st.star` (pre_s `st.star` pre_f)) (st.heap_of_mem m0))
   (ensures
-    (lpreF (st.heap_of_mem m0) <==> lpreF (st.heap_of_mem m1)) /\
+    (lpre_f (st.heap_of_mem m0) <==> lpre_f (st.heap_of_mem m1)) /\
     (forall (x:a) (final_state:st.heap).
-       lpostF (st.heap_of_mem m0) x final_state <==>
-       lpostF (st.heap_of_mem m1) x final_state))
-= frame_post_for_par_tautology lpostF m0;
-  frame_post_for_par_aux preS postS m0 m1 lpostF
+       lpost_f (st.heap_of_mem m0) x final_state <==>
+       lpost_f (st.heap_of_mem m1) x final_state))
+= frame_post_for_par_tautology lpost_f m0;
+  frame_post_for_par_aux pre_s post_s m0 m1 lpost_f
 
 
 /// Finally lemmas for proving that in the par rules preconditions get weaker
 ///   and postconditions get stronger
 
-#push-options "--z3rlimit 100"
 let par_weaker_pre_and_stronger_post_l (#st:st) (#preL:st.hprop) (lpreL:l_pre preL)
   (#aL:Type) (#postL:post st aL) (lpostL:l_post preL postL)
   (#next_preL:st.hprop) (next_lpreL:l_pre next_preL) (next_lpostL:l_post next_preL postL)
@@ -687,7 +652,44 @@ let par_weaker_pre_and_stronger_post_l (#st:st) (#preL:st.hprop) (lpreL:l_pre pr
       (par_lpost next_lpreL next_lpostL lpreR lpostR)
       state next_state)
 = frame_post_for_par preL next_preL state next_state lpreR lpostR;
-  assert (weaker_pre (par_lpre lpreL lpreR) (par_lpre next_lpreL lpreR) state next_state)
+  assert (weaker_pre (par_lpre lpreL lpreR) (par_lpre next_lpreL lpreR) state next_state) by
+    (norm [delta_only [`%weaker_pre; `%par_lpre] ])
+
+let commute_star_right (#st:st) (p q r:st.hprop)
+: Lemma
+  ((p `st.star` (q `st.star` r)) `st.equals`
+   (p `st.star` (r `st.star` q)))
+= calc (st.equals) {
+    p `st.star` (q `st.star` r);
+       (st.equals) { equals_ext_right p (q `st.star` r) (r `st.star` q) }
+    p `st.star` (r `st.star` q);
+  }
+
+let assoc_star_right (#st:st) (p q r s:st.hprop)
+: Lemma
+  ((p `st.star` ((q `st.star` r) `st.star` s)) `st.equals`
+   (p `st.star` (q `st.star` (r `st.star` s))))
+= calc (st.equals) {
+    p `st.star` ((q `st.star` r) `st.star` s);
+       (st.equals) { equals_ext_right p ((q `st.star` r) `st.star` s)
+                                        (q `st.star` (r `st.star` s)) }
+    p `st.star` (q `st.star` (r `st.star` s));
+  }
+
+let commute_assoc_star_right (#st:st) (p q r s:st.hprop)
+: Lemma
+  ((p `st.star` ((q `st.star` r) `st.star` s)) `st.equals`
+   (p `st.star` (r `st.star` (q `st.star` s))))
+= admit ()
+
+
+let apply_interp_ext (#st:st) (p q:st.hprop) (m:st.mem)
+: Lemma
+  (requires
+    st.interp p (st.heap_of_mem m) /\
+    p `st.equals` q)
+  (ensures st.interp q (st.heap_of_mem m))
+= ()
 
 let par_weaker_pre_and_stronger_post_r (#st:st) (#preL:st.hprop) (lpreL:l_pre preL)
   (#aL:Type) (#postL:post st aL) (lpostL:l_post preL postL)
@@ -705,6 +707,7 @@ let par_weaker_pre_and_stronger_post_r (#st:st) (#preL:st.hprop) (lpreL:l_pre pr
     lpreL (st.heap_of_mem state) /\
     st.interp (st.locks_invariant state `st.star` (preL `st.star` preR)) (st.heap_of_mem state))
   (ensures
+    st.interp (st.locks_invariant next_state `st.star` (preL `st.star` next_preR)) (st.heap_of_mem next_state) /\
     weaker_pre
       (par_lpre lpreL lpreR)
       (par_lpre lpreL next_lpreR)
@@ -713,10 +716,19 @@ let par_weaker_pre_and_stronger_post_r (#st:st) (#preL:st.hprop) (lpreL:l_pre pr
       (par_lpost lpreL lpostL lpreR lpostR)
       (par_lpost lpreL lpostL next_lpreR next_lpostR)
       state next_state)
-= assume (st.interp (st.locks_invariant state `st.star` (preR `st.star` preL)) (st.heap_of_mem state));
+= commute_star_right (st.locks_invariant state) preL preR;
+  apply_interp_ext
+    (st.locks_invariant state `st.star` (preL `st.star` preR))
+    (st.locks_invariant state `st.star` (preR `st.star` preL))
+    state;
   frame_post_for_par preR next_preR state next_state lpreL lpostL;
-  assert (weaker_pre (par_lpre lpreL lpreR) (par_lpre lpreL next_lpreR) state next_state)
-#pop-options
+  assert (weaker_pre (par_lpre lpreL lpreR) (par_lpre lpreL next_lpreR) state next_state) by
+    (norm [delta_only [`%weaker_pre; `%par_lpre] ]);
+  commute_star_right (st.locks_invariant next_state) next_preR preL;
+  apply_interp_ext
+    (st.locks_invariant next_state `st.star` (next_preR `st.star` preL))
+    (st.locks_invariant next_state `st.star` (preL `st.star` next_preR))
+    next_state
 
 (**** Begin stepping functions ****)
 
@@ -728,9 +740,14 @@ let step_ret (#st:st) (i:nat) (#a:Type u#a)
 : Div (step_result a post) (step_req f state) (step_ens f state)
 
 = let Ret p x lp = f in
-  Step state (p x) (p x) state lpre lpost f i
+  Step (p x) state (p x) state lpre lpost f i
 
-#push-options "--z3rlimit 100"
+
+let lpost_ret_act (#st:st) (#a:Type) (#pre:st.hprop) (#post:post st a) (lpost:l_post pre post)
+  (x:a) (state:st.mem)
+: l_post (post x) post
+= fun _ x h1 -> lpost (st.heap_of_mem state) x h1
+
 let step_act (#st:st) (i:nat)
   (#a:Type u#a) (#pre:st.hprop) (#post:post st a) (#lpre:l_pre pre) (#lpost:l_post pre post)
   (f:m st a pre post lpre lpost{Act? f})
@@ -738,16 +755,14 @@ let step_act (#st:st) (i:nat)
 
 : Div (step_result a post) (step_req f state) (step_ens f state)
 
-= let Act #_ #_ #_ #_ #_ #lpost f = f in
+= let Act #_ #_ #_ #_ #_ #_ f = f in
 
-  let x, new_state = f state in
+  let x, next_state = f state in
 
-  let lpost : l_post (post x) post = fun _ x h1 -> lpost (st.heap_of_mem state) x h1 in
-  Step state pre (post x) new_state (fun h -> lpost h x h) lpost (Ret post x lpost) i
-#pop-options
+  let lpost : l_post (post x) post = lpost_ret_act lpost x state in
 
-#restart-solver
-#set-options "--z3rlimit 100"
+  Step pre state (post x) next_state (fun h -> lpost h x h) lpost (Ret post x lpost) i
+
 let step_bind (#st:st) (i:nat)
   (#a:Type u#a) (#pre:st.hprop) (#post:post st a) (#lpre:l_pre pre) (#lpost:l_post pre post)
   (f:m st a pre post lpre lpost{Bind? f})
@@ -758,25 +773,60 @@ let step_bind (#st:st) (i:nat)
 
 = match f with
   | Bind #_ #_ #_ #_ #_ #_ #_ #_ #lpre_b #lpost_b (Ret p x _) g ->
-    Step state (p x) (p x) state (lpre_b x) (lpost_b x) (g x) i
+    Step (p x) state (p x) state (lpre_b x) (lpost_b x) (g x) i
 
-  | Bind #_ #_ #_ #_ #_ #_ #_ #_ #lpre_b #lpost_b f g ->
-    let Step state pre_a next_pre next_state next_lpre next_lpost f j = step i f state in
-    
-    Step state pre_a next_pre next_state
+  | Bind #_ #_ #pre_a #_ #lpre_a #lpost_a #_ #_ #lpre_b #lpost_b f g ->
+    let Step pre_a state1 next_pre next_state next_lpre next_lpost f j = step i f state in
+
+    assert (bind_lpre next_lpre next_lpost lpre_b (st.heap_of_mem next_state)) by
+      norm ([delta_only [`%bind_lpre]]);
+
+    Step pre_a state1 next_pre next_state
       (bind_lpre next_lpre next_lpost lpre_b)
       (bind_lpost next_lpre next_lpost lpost_b)
       (Bind f g)
       j
 
+
+let weaken_fp_prop (#st:st) (frame frame':st.hprop) (m0 m1:st.mem)
+: Lemma
+  (requires
+    forall (f_frame:fp_prop (frame `st.star` frame')).
+      f_frame (st.heap_of_mem m0) <==>
+      f_frame (st.heap_of_mem m1))
+   (ensures
+    forall (f_frame:fp_prop frame').
+      f_frame (st.heap_of_mem m0) <==>
+      f_frame (st.heap_of_mem m1))
+= ()
+    
+#push-options "--z3rlimit 40"
 let preserves_frame_star (#st:st) (pre post:st.hprop) (m0 m1:st.mem) (frame:st.hprop)
 : Lemma
   (requires preserves_frame pre post m0 m1)
   (ensures preserves_frame (pre `st.star` frame) (post `st.star` frame) m0 m1)
-= admit ()
+= let aux (frame':st.hprop)
+    : Lemma
+      (requires
+        st.interp (st.locks_invariant m0 `st.star` ((pre `st.star` frame) `st.star` frame')) (st.heap_of_mem m0))
+      (ensures
+        st.interp (st.locks_invariant m1 `st.star` ((post `st.star` frame) `st.star` frame')) (st.heap_of_mem m1) /\
+        (forall (f_frame:fp_prop frame'). f_frame (st.heap_of_mem m0) <==> f_frame (st.heap_of_mem m1)))
+    = assoc_star_right (st.locks_invariant m0) pre frame frame';
+      apply_interp_ext
+        (st.locks_invariant m0 `st.star` ((pre `st.star` frame) `st.star` frame'))
+        (st.locks_invariant m0 `st.star` (pre `st.star` (frame `st.star` frame')))
+        m0;
+      assoc_star_right (st.locks_invariant m1) post frame frame';
+      apply_interp_ext
+        (st.locks_invariant m1 `st.star` (post `st.star` (frame `st.star` frame')))
+        (st.locks_invariant m1 `st.star` ((post `st.star` frame) `st.star` frame'))
+        m1;
+      weaken_fp_prop frame frame' m0 m1
+  in
+  Classical.forall_intro (Classical.move_requires aux)
+#pop-options
 
-#set-options "--z3rlimit 50"
-#restart-solver
 let step_frame (#st:st) (i:nat)
   (#a:Type u#a) (#pre:st.hprop) (#p:post st a) (#lpre:l_pre pre) (#lpost:l_post pre p)
   (f:m st a pre p lpre lpost{Frame? f})
@@ -787,18 +837,18 @@ let step_frame (#st:st) (i:nat)
 
 = match f with  
   | Frame (Ret p x lp) frame f_frame ->
-    Step state (p x `st.star` frame) (p x `st.star` frame) state
+    Step (p x `st.star` frame) state (p x `st.star` frame) state
       (fun h -> lpost h x h)
       lpost
       (Ret (fun x -> p x `st.star` frame) x lpost)
       i
 
   | Frame #_ #_ #f_pre #_ #f_lpre #f_lpost f frame f_frame ->
-    let Step state pre next_fpre next_state next_flpre next_flpost f j = step i f state in
+    let Step pre state next_fpre next_state next_flpre next_flpost f j = step i f state in
 
     preserves_frame_star pre next_fpre state next_state frame;
 
-    Step state (pre `st.star` frame) (next_fpre `st.star` frame) next_state
+    Step (pre `st.star` frame) state (next_fpre `st.star` frame) next_state
       (frame_lpre next_flpre f_frame)
       (frame_lpost next_flpre next_flpost f_frame)
       (Frame f frame f_frame)
@@ -809,15 +859,33 @@ let step_frame (#st:st) (i:nat)
 
 assume val go_left : nat -> bool
 
+#push-options "--z3rlimit 40"
 let preserves_frame_star_left (#st:st) (pre post:st.hprop) (m0 m1:st.mem) (frame:st.hprop)
 : Lemma
   (requires preserves_frame pre post m0 m1)
   (ensures preserves_frame (frame `st.star` pre) (frame `st.star` post) m0 m1)
-= admit ()
+= let aux (frame':st.hprop)
+    : Lemma
+      (requires
+        st.interp (st.locks_invariant m0 `st.star` ((frame `st.star` pre) `st.star` frame')) (st.heap_of_mem m0))
+      (ensures
+        st.interp (st.locks_invariant m1 `st.star` ((frame `st.star` post) `st.star` frame')) (st.heap_of_mem m1) /\
+        (forall (f_frame:fp_prop frame'). f_frame (st.heap_of_mem m0) <==> f_frame (st.heap_of_mem m1)))
+    = commute_assoc_star_right (st.locks_invariant m0) frame pre frame';
+      apply_interp_ext
+        (st.locks_invariant m0 `st.star` ((frame `st.star` pre) `st.star` frame'))
+        (st.locks_invariant m0 `st.star` (pre `st.star` (frame `st.star` frame')))
+        m0;
+      commute_assoc_star_right (st.locks_invariant m1) frame post frame';
+      apply_interp_ext
+        (st.locks_invariant m1 `st.star` (post `st.star` (frame `st.star` frame')))
+        (st.locks_invariant m1 `st.star` ((frame `st.star` post) `st.star` frame'))
+        m1;
+      weaken_fp_prop frame frame' m0 m1
+  in
+  Classical.forall_intro (Classical.move_requires aux)
+#pop-options
 
-
-#restart-solver
-#push-options "--z3rlimit 150"
 let step_par (#st:st) (i:nat)
   (#a:Type u#a) (#pre:st.hprop) (#post:post st a) (#lpre:l_pre pre) (#lpost:l_post pre post)
   (f:m st a pre post lpre lpost{Par? f})
@@ -831,7 +899,7 @@ let step_par (#st:st) (i:nat)
 
     let lpost : l_post #st #(aL & aR) _ _ = fun h0 (xL, xR) h1 -> lpL h0 xL h1 /\ lpR h0 xR h1 in
 
-    Step state (pL xL `st.star` pR xR) (pL xL `st.star` pR xR) state
+    Step (pL xL `st.star` pR xR) state (pL xL `st.star` pR xR) state
       (fun h -> lpL h xL h /\ lpR h xR h)
       lpost 
       (Ret (fun (xL, xR) -> pL xL `st.star` pR xR) (xL, xR) lpost)
@@ -839,32 +907,29 @@ let step_par (#st:st) (i:nat)
 
   | Par #_ #aL #preL #postL #lpreL #lpostL mL #aR #preR #postR #lpreR #lpostR mR ->
     if go_left i then begin
-      let Step state pre next_preL next_state next_lpreL next_lpostL mL j = step (i + 1) mL state in
+      let Step pre state next_preL next_state next_lpreL next_lpostL mL j = step (i + 1) mL state in
 
       preserves_frame_star pre next_preL state next_state preR;
       par_weaker_pre_and_stronger_post_l lpreL lpostL next_lpreL next_lpostL lpreR lpostR state next_state;
 
-      Step state (pre `st.star` preR) (next_preL `st.star` preR) next_state
+      Step (pre `st.star` preR) state (next_preL `st.star` preR) next_state
         (par_lpre next_lpreL lpreR)
         (par_lpost next_lpreL next_lpostL lpreR lpostR)
         (Par mL mR)
         j
     end
     else begin
-      let Step state pre next_preR next_state next_lpreR next_lpostR mR j = step (i + 1) mR state in
+      let Step pre state next_preR next_state next_lpreR next_lpostR mR j = step (i + 1) mR state in
 
       preserves_frame_star_left pre next_preR state next_state preL;
       par_weaker_pre_and_stronger_post_r lpreL lpostL lpreR lpostR next_lpreR next_lpostR state next_state;
 
-      assume (st.interp (st.locks_invariant next_state `st.star` (preL `st.star` next_preR)) (st.heap_of_mem next_state));
-
-      Step state (preL `st.star` pre) (preL `st.star` next_preR) next_state
+      Step (preL `st.star` pre) state (preL `st.star` next_preR) next_state
         (par_lpre lpreL next_lpreR)
         (par_lpost lpreL lpostL next_lpreR next_lpostR)
         (Par mL mR)
         j
     end
-#pop-options
 
 let step_weaken (#st:st) (i:nat) (#a:Type u#a)
   (#pre:st.hprop) (#post:post st a) (#lpre:l_pre pre) (#lpost:l_post pre post)
@@ -875,7 +940,7 @@ let step_weaken (#st:st) (i:nat) (#a:Type u#a)
 
 = let Weaken #_ #_ #pre #post #lpre #lpost #_ #_ #_ f = f in
 
-  Step state pre pre state lpre lpost f i
+  Step pre state pre state lpre lpost f i
 
 
 /// Step function
@@ -887,19 +952,13 @@ let rec step (#st:st) (i:nat) (#a:Type u#a)
 : Div (step_result a post)
   (step_req f state)
   (step_ens f state)
-= admit ()
-
-  // fun #st i #a #pre #post #o_lpre #o_lpost frame f state ->
-  // match f with
-  // | Ret _ _ _   ->    step_ret i frame f state
-  // | Act _ _ _   ->    step_act i frame f state
-  // | Bind _ _    ->   step_bind i frame f state step
-  // | Frame _ _ _ ->  step_frame i frame f state step
-  // | Par _ _     ->    step_par i frame f state step
-  // | Weaken _    -> step_weaken i frame f state
-
-
-/// Top-level run function
+= match f with
+  | Ret _ _ _ -> step_ret i f state
+  | Bind _ _ -> step_bind i f state step
+  | Act _ -> step_act i f state
+  | Frame _ _ _ -> step_frame i f state step
+  | Par _ _ -> step_par i f state step
+  | Weaken _ -> step_weaken i f state
 
 let rec run (#st:st) (i:nat) (#a:Type u#a) (#pre:st.hprop) (#post:post st a)
   (#lpre:l_pre pre) (#lpost:l_post pre post)
@@ -923,36 +982,36 @@ let rec run (#st:st) (i:nat) (#a:Type u#a) (#pre:st.hprop) (#post:post st a)
     (x, final_state)
 
 
-// (**** Trying to define the layered effect ****)
+// // (**** Trying to define the layered effect ****)
 
-// type repr (a:Type) (st:st) (pre:st.hprop) (post:post st a) (lpre:l_pre pre) (lpost:l_post pre post)
-// = unit -> m st a pre post lpre lpost
+// // type repr (a:Type) (st:st) (pre:st.hprop) (post:post st a) (lpre:l_pre pre) (lpost:l_post pre post)
+// // = unit -> m st a pre post lpre lpost
 
 
-// /// This will not be allowed currently as the extra binders must appear before x in the implementation, can change
+// // /// This will not be allowed currently as the extra binders must appear before x in the implementation, can change
 
-// let return (a:Type) (st:st) (post:post st a) (lpost:(x:a -> l_post (post x) post)) (x:a)
-// : repr a st (post x) post (fun h -> (lpost x) h x h) (lpost x)
-// = fun _ -> Ret post x (lpost x)
+// // let return (a:Type) (st:st) (post:post st a) (lpost:(x:a -> l_post (post x) post)) (x:a)
+// // : repr a st (post x) post (fun h -> (lpost x) h x h) (lpost x)
+// // = fun _ -> Ret post x (lpost x)
 
-// let bind (a:Type) (b:Type) (st:st)
-//   (pre_f:st.hprop) (post_f:post st a) (lpre_f:l_pre pre_f) (lpost_f:l_post pre_f post_f)
-//   (post_g:post st b) (lpre_g:(x:a -> l_pre (post_f x))) (lpost_g:(x:a -> l_post (post_f x) post_g))
-//   (f:repr a st pre_f post_f lpre_f lpost_f)
-//   (g:(x:a -> repr b st (post_f x) post_g (lpre_g x) (lpost_g x)))
-// : repr b st pre_f post_g
-//     (bind_lpre lpre_f lpost_f lpre_g)
-//     (bind_lpost lpre_f lpost_f lpost_g)
-// = fun _ -> Bind (f ()) (fun x -> g x ())
+// // let bind (a:Type) (b:Type) (st:st)
+// //   (pre_f:st.hprop) (post_f:post st a) (lpre_f:l_pre pre_f) (lpost_f:l_post pre_f post_f)
+// //   (post_g:post st b) (lpre_g:(x:a -> l_pre (post_f x))) (lpost_g:(x:a -> l_post (post_f x) post_g))
+// //   (f:repr a st pre_f post_f lpre_f lpost_f)
+// //   (g:(x:a -> repr b st (post_f x) post_g (lpre_g x) (lpost_g x)))
+// // : repr b st pre_f post_g
+// //     (bind_lpre lpre_f lpost_f lpre_g)
+// //     (bind_lpost lpre_f lpost_f lpost_g)
+// // = fun _ -> Bind (f ()) (fun x -> g x ())
 
-// let subcomp (a:Type) (st:st)
-//   (pre:st.hprop) (post:post st a)
-//   (lpre_f:l_pre pre) (lpost_f:l_post pre post)
-//   (lpre_g:l_pre pre) (lpost_g:l_post pre post)
-//   (f:repr a st pre post lpre_f lpost_f)
-// : Pure (repr a st pre post lpre_g lpost_g)
-//   (requires
-//     (forall h. lpre_g h ==> lpre_f h) /\
-//     (forall h0 x h1. lpost_f h0 x h1 ==> lpost_g h0 x h1))
-//   (ensures fun _ -> True)
-// = fun _ -> Weaken #_ #a #pre #post #lpre_f #lpost_f #lpre_g #lpost_g #() (f ())
+// // let subcomp (a:Type) (st:st)
+// //   (pre:st.hprop) (post:post st a)
+// //   (lpre_f:l_pre pre) (lpost_f:l_post pre post)
+// //   (lpre_g:l_pre pre) (lpost_g:l_post pre post)
+// //   (f:repr a st pre post lpre_f lpost_f)
+// // : Pure (repr a st pre post lpre_g lpost_g)
+// //   (requires
+// //     (forall h. lpre_g h ==> lpre_f h) /\
+// //     (forall h0 x h1. lpost_f h0 x h1 ==> lpost_g h0 x h1))
+// //   (ensures fun _ -> True)
+// // = fun _ -> Weaken #_ #a #pre #post #lpre_f #lpost_f #lpre_g #lpost_g #() (f ())
